More proof work and semantic refactor
Found some too strong general semantic parts that needed refactor so the proof work could be done. Only four axioms remain in the internal language lemma files and also got some progress in the translation lemma files.

src/machine_inter.v
@@ -111,7 +111,7 @@ Fixpoint expr_subst (x : string) (s : i_expr) (e : i_expr) : i_expr :=
   | ENat n => ENat n
   | EUnit u => EUnit u
   | EFix f y τ₁ τ₂ body =>
-    if String.eqb f x || String.eqb y x then EFix f y τ₁ τ₂ body
+    if String.eqb y x then EFix f y τ₁ τ₂ body
     else EFix f y τ₁ τ₂ (expr_subst x s body)
   | EApp e1 e2 => EApp (expr_subst x s e1) (expr_subst x s e2)
   | EPlus e1 e2 => EPlus (expr_subst x s e1) (expr_subst x s e2)
@@ -196,7 +196,7 @@ Inductive step : (ctx * i_expr) -> (ctx * i_expr) -> Prop :=
       value Γ v ->
       step
         (Γ, EApp (EFix f x τ₁ τ₂ e) v)
-        (Γ, expr_subst f (EFix f x τ₁ τ₂ e) (expr_subst x v e))
+        (Γ, expr_subst_fun f (EFix f x τ₁ τ₂ e) (expr_subst x v e))
   | StepFst :
     forall Γ v₁ v₂,
       value Γ v₁ ->
